TouhouFormal/Search.lean
@@ -9,6 +9,7 @@ import TouhouFormal.Search.IntUnaryUpdate
 import TouhouFormal.Search.Movement
 import TouhouFormal.Search.EnemyState
 import TouhouFormal.Search.Shooting
+import TouhouFormal.Search.BulletPattern
 import TouhouFormal.Search.Random
 import TouhouFormal.Search.ScalarAssignment
 import TouhouFormal.Search.SMT
